contracts/verification/easycrypt/c10-port/cdrafts-split/C10DigitUniform.ec
@@ -1,0 +1,89 @@
+(* Exact acceptance arithmetic for an independently uniform bit string.
+   This file makes no assumption about SHA-256 outputs or counter searches. *)
+require import AllCore List Distr DList DBool BitEncoding IntDiv StdOrder.
+require import CountDS RadixEncoding.
+import BS2Int IntOrder RealOrder.
+
+lemma uniform_same_support ['a] (d e : 'a distr) :
+  is_uniform d => is_uniform e => is_lossless d => is_lossless e =>
+  (forall x, (x \in d) = (x \in e)) => d = e.
+proof.
+  move=> du eu dl el hs.
+  have he : support d = support e by apply fun_ext => x; apply hs.
+  by apply eq_distr => x; rewrite !mu1_uni // dl el he.
+qed.
+
+lemma pow2_3 : 2 ^ 3 = 8.
+proof. by rewrite (_ : 3 = 2 + 1) 1:// exprS 1://
+  (_ : 2 = 1 + 1) 1:// exprS 1:// expr1. qed.
+
+lemma uniform_three_bits : dmap (dlist dbool 3) bs2int = drange 0 8.
+proof.
+  apply uniform_same_support.
+  + apply dmap_uni_in_inj.
+    - move=> x y hx hy hxy; apply inj_bs2int_eqsize; last exact hxy.
+      by rewrite (supp_dlist_size dbool 3 x _ hx) 1://
+                 (supp_dlist_size dbool 3 y _ hy) 1://.
+    exact (dlist_uni _ _ dbool_uni).
+  + exact drange_uni.
+  + apply dmap_ll; exact (dlist_ll _ _ dbool_ll).
+  + by apply drange_ll.
+  move=> x; rewrite supp_dmap supp_drange eq_iff; split.
+  + move=> [bs [hbs ->]]; have hs := supp_dlist_size dbool 3 bs _ hbs; first done.
+    have := bs2int_le2Xs bs; rewrite hs pow2_3; smt(bs2int_ge0).
+  move=> hx; exists (int2bs 3 x); split.
+  + rewrite supp_dlist 1:// size_int2bs ler_maxr 1:// /=.
+    apply allP => b hb.
+    exact supp_dbool.
+  by rewrite int2bsK 1:// 1:pow2_3.
+qed.
+
+lemma size_words (n b : int) : 0 <= n => 0 <= b =>
+  size (words n b) = b ^ n.
+proof.
+  move=> hn hb; elim: n hn => [|n hn ih].
+  + by rewrite words0 /= expr0.
+  by rewrite wordsS // size_allpairs size_range ler_maxr 1:/#
+    ih exprS //; ring.
+qed.
+
+lemma uniform_words (n b : int) : 0 <= n => 0 < b =>
+  dlist (drange 0 b) n = duniform (words n b).
+proof.
+  move=> hn hb; apply uniform_same_support.
+  + exact (dlist_uni _ _ (drange_uni 0 b)).
+  + exact duniform_uni.
+  + apply dlist_ll; exact (drange_ll 0 b hb).
+  + apply duniform_ll; have := size_words n b hn _; first smt().
+    have hp : 0 < b ^ n by apply IntOrder.expr_gt0.
+    smt(size_eq0).
+  move=> l; rewrite supp_dlist // supp_duniform mem_words //.
+  have hp : support (drange 0 b) = is_digit b.
+  + by apply fun_ext => d; rewrite supp_drange /is_digit.
+  by rewrite hp.
+qed.
+
+lemma uniform_digits (n extra : int) : 0 <= n => 0 <= extra =>
+  dmap (dlist dbool (3*n+extra)) (digits 3 n) = dlist (drange 0 8) n.
+proof.
+  move=> hn he; elim: n hn => [|n hn ih].
+  + rewrite (dlist0 (drange 0 8) 0) 1:// (_ : digits 3 0 = fun _ => []).
+    - by apply fun_ext => bs; rewrite /digits mkseq0.
+    by rewrite dmap_cst //; apply dlist_ll; exact dbool_ll.
+  rewrite (_ : 3*(n+1)+extra = 3+(3*n+extra)) 1:/# dlist_add 1:// 1:/# dmap_comp.
+  rewrite (eq_dmap_in _ _ (fun xy : bool list * bool list => bs2int xy.`1 :: digits 3 n xy.`2)).
+  + move=> [lo hi] /= /supp_dprod [hlo hhi]; rewrite /(\o) /= digits_cat //.
+    exact (supp_dlist_size dbool 3 lo _ hlo).
+  by rewrite (dmap_dprod_comp _ _ bs2int (digits 3 n) (fun x xs => x :: xs))
+    uniform_three_bits ih dlistS.
+qed.
+
+lemma uniform_digit_sum (n extra target : int) : 0 <= n => 0 <= extra =>
+  mu (dlist dbool (3*n+extra)) (fun bs => sumz (digits 3 n bs) = target)
+   = (count_ds n 8 target)%r / (8 ^ n)%r.
+proof.
+  move=> hn he.
+  rewrite -(dmapE (dlist dbool (3*n+extra)) (digits 3 n) (fun ds => sumz ds = target)).
+  by rewrite uniform_digits // uniform_words // duniformE undup_id 1:uniq_words //
+    -count_ds_correct // size_words.
+qed.
